formal/inference/InferenceTest.thy
@@ -1,454 +1,545 @@
 theory InferenceTest
-imports Learn_EFSM Trace_Matches Increment_Reset Code_Generation
+imports Trace_Matches Increment_Reset Code_Generation InferenceTestEFSMs
 begin
 
-declare One_nat_def [simp del]
-
-definition "heuristics = try_heuristics [heuristic_1 traces, insert_increment]"
+definition "heuristics = iterative_try_heuristics [(\<lambda>x. insert_increment), (\<lambda>x. heuristic_1 x)]"
 
 termination infer sorry
 termination resolve_nondeterminism sorry
 
-abbreviation "coin_general \<equiv> \<lparr>Label = STR ''coin'', Arity = 1, Guard = [], Outputs = [Plus (V (R 1)) (V (I 1))], Updates = [(R 1, Plus (V (R 1)) (V (I 1)))]\<rparr>"
-abbreviation "vend_initialise \<equiv> \<lparr>Label = STR ''vend'', Arity = 0, Guard = [], Outputs = [L (value.Str STR ''pepsi'')], Updates = [(R 1, L (Num 0))]\<rparr>"
-abbreviation "coin50_initialise \<equiv> \<lparr>Label = STR ''coin'', Arity = 1, Guard = [gexp.Eq (V (I 1)) (L (Num 50))], Outputs = [L (Num 100)], Updates = [(R 1, L (Num 0))]\<rparr>"
+lemma tm_same: "x = y \<Longrightarrow> tm x = tm y"
+  by simp
 
-definition "heuristics_2_9 = {|(0, (0, 1), select coke),
-     (1, (0, 7), select pepsi),
-     (2, (1, 2), coin_general),
-     (3, (1, 5), coin 100 100),
-     (4, (2, 3), coin50_initialise),
-     (5, (3, 4), vend coke),
-     (6, (5, 6), vend coke),
-     (7, (7, 1), coin_general),
-     (8, (1, 2), coin_general),
-     (9, (2, 10), vend_initialise)|}"
+definition "first_trace = [((STR ''select''), [(Str ''coke'')], []), ((STR ''coin''), [Num 50], [Num 50]), ((STR ''coin''), [Num 50], [Num 100]), ((STR ''vend''), [], [(Str ''coke'')])]"
+definition "second_trace = [((STR ''select''), [(Str ''coke'')], []), ((STR ''coin''), [Num 100], [Num 100]), ((STR ''vend''), [], [(Str ''coke'')])]"
+definition "third_trace = [((STR ''select''), [(Str ''pepsi'')], []), ((STR ''coin''), [Num 50], [Num 50]), ((STR ''coin''), [Num 50], [Num 100]), ((STR ''vend''), [], [(Str ''pepsi'')])]"
 
-lemma choice_coin_specific_coin_general:"choice (coin m n) coin_general"
-  apply (simp add: choice_def)
-  by auto
+lemma traces_alt: "traces = [first_trace, second_trace, third_trace]"
+  by (simp add: first_trace_def second_trace_def third_trace_def traces_def)
 
-lemma nondeterministic_pairs_heuristics_2_9: "nondeterministic_pairs heuristics_2_9 = {|
-(1, (2, 5), (coin_general, 8), coin 100 100, 3),
-(1, (2, 2), (coin_general, 8), coin_general, 2),
-(1, (5, 2), (coin 100 100, 3), coin_general, 8),
-(1, (5, 2), (coin 100 100, 3), coin_general, 2),
-(1, (2, 2), (coin_general, 2), coin_general, 8),
-(1, (2, 5), (coin_general, 2), coin 100 100, 3)
+lemma first_branch: "toiEFSM (make_branch (tm {||}) 0 Map.empty first_trace) = first_branch"
+  by eval
+
+lemma score_first_branch: "sorted_list_of_fset (score (first_branch) naive_score) = [(1, 1, 2)]"
+  by eval
+
+lemma merge_1_2: "merge_states 1 2 first_branch = merge_1_2"
+  by eval
+
+lemma nondeterministic_pairs: "ffUnion (fimage (\<lambda>s. state_nondeterminism s (outgoing_transitions s t)) (S t)) = sn \<Longrightarrow>
+                                ffilter (\<lambda>(_, (d1, d2), t, t'). choice (fst t) (fst t')) sn = nd \<Longrightarrow>
+                                nondeterministic_pairs t = nd"
+  by (simp add: nondeterministic_pairs_def)
+
+lemma nondeterministic_pairs_merge_1_2: "nondeterministic_pairs merge_1_2 = {|(1, (1, 3), (coin 50 50, 1), coin 50 100, 2), (1, (3, 1), (coin 50 100, 2), coin 50 50, 1)|}"
+proof-
+  have union: "ffUnion ((\<lambda>s. state_nondeterminism s (outgoing_transitions s merge_1_2)) |`| Inference.S merge_1_2) = {|(1, (1, 3), (coin 50 50, 1), coin 50 100, 2), (1, (3, 1), (coin 50 100, 2), coin 50 50, 1)|}"
+    by eval
+  show ?thesis
+    apply (rule nondeterministic_pairs)
+     apply (simp add: union)
+    apply (simp add: Abs_ffilter Set.filter_def)
+    using choice_def
+    by auto
+qed
+
+lemma merge_3_1: "merge_states 3 1 merge_1_2 = merge_3_1"
+  by eval
+
+lemma merge_transitions_heuristic: "\<not> directly_subsumes (tm oldEFSM) (tm newEFSM) t1FromOld t2 t1 \<Longrightarrow>
+       \<not> directly_subsumes (tm oldEFSM) (tm newEFSM) t2FromOld t1 t2 \<Longrightarrow>
+       m u1 u2 newFrom newEFSM oldEFSM = Some e \<Longrightarrow>
+       merge_transitions oldEFSM newEFSM t1FromOld t2FromOld newFrom t1NewTo t2NewTo t1 u1 t2 u2 m = Some e"
+  by (simp add: merge_transitions_def)
+
+lemma merge_transitions_coin_50: "merge_transitions first_branch merge_3_1 2 1 1 1 1 (coin 50 100) 2 (coin 50 50) 1 (heuristics [first_trace]) = Some first_branch_initialise"
+  apply (rule merge_transitions_heuristic)
+  using coin_50_50_cant_directly_subsume_coin_50_100 apply blast
+  using coin_50_100_cant_directly_subsume_coin_50_50 apply blast
+  by eval
+
+lemma Abs_fset_both_sides: "finite s \<Longrightarrow> (fset f = s) = (f = Abs_fset s)"
+  apply standard
+  using fset_inverse apply fastforce
+  by (simp add: Abs_fset_inverse)
+
+lemma nondeterministic_pairs_first_branch_initialise: "nondeterministic_pairs first_branch_initialise = {||}"
+proof-
+  have state_nondeterminism: "ffUnion ((\<lambda>s. state_nondeterminism s (outgoing_transitions s first_branch_initialise)) |`| Inference.S first_branch_initialise) =
+    {|(1, (1, 4), (coin_general 1, 2), vend coke, 3), (1, (4, 1), (vend coke, 3), coin_general 1, 2)|}"
+    by eval
+  show ?thesis
+    apply (rule nondeterministic_pairs)
+     apply (simp only: state_nondeterminism)
+    apply (simp add: Abs_ffilter fset Set.filter_def)
+    using choice_def by auto
+qed
+
+lemma merge_first_branch_1_2: "merge first_branch 1 2 (heuristics [first_trace]) (satisfies {first_trace}) = Some first_branch_initialise"
+proof-
+  have arrives_2_merge_1_2: "arrives 2 merge_1_2 = 3"
+    by eval
+  have arrives_1_merge_1_2: "arrives 1 merge_1_2 = 1"
+    by eval
+  have leaves_2_first_branch: "leaves 2 first_branch = 2"
+    by eval
+  have leaves_1_first_branch: "leaves 1 first_branch = 1"
+    by eval
+  have leaves_2_merge_3_1: "leaves 2 merge_3_1 = 1"
+    by eval
+  have arrives_2_merge_3_1: "arrives 2 merge_3_1 = 1"
+    by eval
+  have arrives_1_merge_3_1: "arrives 1 merge_3_1 = 1"
+    by eval
+  have first_branch_initialise_ok: "satisfies {first_trace} (tm first_branch_initialise)"
+    by eval
+  show ?thesis
+    apply (simp add: merge_def merge_1_2 nondeterministic_pairs_merge_1_2 sorted_list_of_fset_def)
+    apply (simp add:arrives_2_merge_1_2 arrives_1_merge_1_2 merge_3_1)
+    apply (simp add:leaves_2_first_branch leaves_1_first_branch leaves_2_merge_3_1 arrives_2_merge_3_1 arrives_1_merge_3_1)
+    apply (simp add: merge_transitions_coin_50)
+    apply (simp add: deterministic_def nondeterministic_pairs_first_branch_initialise)
+    by (simp add:first_branch_initialise_ok)
+qed
+
+lemma score_first_branch_initialise: "score first_branch_initialise naive_score = {||}"
+  by eval
+
+lemma second_branch: "toiEFSM (make_branch (tm first_branch_initialise) 0 Map.empty second_trace) = second_branch"
+  by eval
+
+lemma score_second_branch: "score second_branch naive_score = {||}"
+  by eval
+
+lemma third_branch: "toiEFSM (make_branch (tm second_branch) 0 Map.empty third_trace) = third_branch"
+  by eval
+
+lemma score_third_branch: "sorted_list_of_fset (score third_branch naive_score) = [(1, 1, 5), (1, 1, 6), (1, 1, 7), (1, 5, 6)]"
+  by eval
+
+lemma merge_5_6: "merge_states 5 6 third_branch = merge_5_6"
+  by eval
+
+lemma nondeterministic_pairs_merge_5_6: "(nondeterministic_pairs merge_5_6) = {|
+(5, (5, 7), (coin 50 50, 4), coin 50 100, 5),
+(5, (7, 5), (coin 50 100, 5), coin 50 50, 4)
 |}"
 proof-
-  have state_nondeterminism_1: "state_nondeterminism 1 {|(2, coin_general, 2), (5, coin 100 100, 3), (2, coin_general, 8)|} = {|(1, (2, 5), (coin_general, 8), coin 100 100, 3), (1, (2, 2), (coin_general, 8), coin_general, 2),
-   (1, (5, 2), (coin 100 100, 3), coin_general, 8), (1, (5, 2), (coin 100 100, 3), coin_general, 2),
-   (1, (2, 2), (coin_general, 2), coin_general, 8), (1, (2, 5), (coin_general, 2), coin 100 100, 3)|}"
+  have union: "ffUnion ((\<lambda>s. state_nondeterminism s (outgoing_transitions s merge_5_6)) |`| Inference.S merge_5_6) = {|(5, (5, 7), (coin 50 50, 4), coin 50 100, 5), (5, (7, 5), (coin 50 100, 5), coin 50 50, 4), (1, (1, 4), (coin_general 1, 2), vend coke, 3),
+   (1, (4, 1), (vend coke, 3), coin_general 1, 2), (0, (1, 5), (select_initialise coke 1, 0), select pepsi, 1),
+   (0, (5, 1), (select pepsi, 1), select_initialise coke 1, 0)|}"
     by eval
-  have state_nondeterminism_2: "state_nondeterminism 2
-                                                       {|(3, \<lparr>Label = STR ''coin'', Arity = 1, Guard = [gexp.Eq (V (I 1)) (L (Num 50))],
-                                                                Outputs = [L (Num 100)], Updates = [(R 1, L (Num 0))]\<rparr>,
-                                                          4),
-                                                         (10,
-                                                          \<lparr>Label = STR ''vend'', Arity = 0, Guard = [],
-                                                             Outputs = [L (value.Str STR ''pepsi'')], Updates = [(R 1, L (Num 0))]\<rparr>,
-                                                          9)|} =  {|(2, (10, 3), (vend_initialise, 9),
-    coin50_initialise, 4),
-   (2, (3, 10),
-    (coin50_initialise, 4),
-    vend_initialise, 9)|}"
-    by eval
-  have state_nondeterminism_0:  "state_nondeterminism 0 {|(1, select coke, 0), (7, select pepsi, 1)|} = {|(0, (7, 1),
-    (select pepsi, 1),
-    select coke, 0),
-   (0, (1, 7), (select coke, 0),
-    select pepsi, 1)|}"
-  by eval
+  have no_choice: "\<not>choice (select_initialise coke 1) (select pepsi)"
+    by (simp add: choice_def)
   show ?thesis
-    apply (simp add: nondeterministic_pairs_def S_def heuristics_2_9_def)
-    apply (simp add: outgoing_transitions_def fimage_def)
-    apply (simp add: state_nondeterminism_1 state_nondeterminism_2 state_nondeterminism_0)
+  apply (rule nondeterministic_pairs)
+     apply (simp only: union)
     apply (simp add: Abs_ffilter Set.filter_def)
     apply standard
      apply clarify
      apply simp
-     apply (case_tac "ab = coin_general")
-      apply simp
-      apply (case_tac "ac = coin 100 100")
-       apply auto[1]
-      apply auto[1]
-     apply (case_tac "ab = vend_initialise")
-      apply (simp add: choice_def)
-     apply (case_tac "ab = coin50_initialise")
-      apply (simp add: choice_def)
-     apply (case_tac "ab = coin 100 100")
-      apply (case_tac "ac = coin_general")
-       apply (simp add: choice_def)
-       apply auto[1]
-      apply simp
-     apply (case_tac "ab = vend_initialise")
+     apply (case_tac "ab = coin 50 50")
       apply simp
      apply simp
-     apply (meson choice_symmetry no_choice_select_coke_select_pepsi)
-    apply clarify
-    apply simp
-    apply (case_tac "ab = coin_general")
-     apply (case_tac "ac = coin_general")
-      apply (simp add: choice_def)
-     apply (case_tac "ac = coin 100 100")
-      apply (simp add: choice_def)
-      apply auto[1]
+     apply (case_tac "ab = coin 50 100")
+      apply simp
      apply simp
-    apply simp
-    using choice_coin_specific_coin_general by blast
+     apply (case_tac "ab = coin_general 1")
+      apply (simp add: choice_def)
+     apply simp
+     apply (case_tac "ab = vend coke")
+      apply (simp add: choice_def)
+     apply simp
+     apply (case_tac "ab = select_initialise coke 1")
+      apply (simp add: no_choice)
+     apply (simp add: no_choice choice_symmetry)
+    using choice_def by auto
 qed
 
-definition "merge_5_2 = {|
-(0, (0, 1), select coke),
-   (1, (0, 7), select pepsi),
-   (2, (1, 2), coin_general), (3, (1, 2), coin 100 100), (4, (2, 3), coin50_initialise),
-   (5, (3, 4), vend coke),
-   (6, (2, 6), vend coke),
-   (7, (7, 1), coin_general), (8, (1, 2), coin_general), (9, (2, 10), vend_initialise)|}"
-
-lemma merge_5_2: "merge_states 5 2 heuristics_2_9 = merge_5_2 \<and> merge_states 2 5 heuristics_2_9 = merge_5_2"
+lemma merge_7_5: "merge_states 7 5 merge_5_6 = merge_7_5"
   by eval
 
-lemma step_pta_select_pepsi: "step (tm pta) 0 Map.empty (STR ''select'') [(Str ''pepsi'')] = Some ((select pepsi), 7, [], <>)"
-  apply (rule one_possible_step)
-    apply (rule possible_steps_singleton)
-    apply (simp add: Abs_ffilter Set.filter_def pta_def tm_def)
-  using implode_coke implode_pepsi
-  by auto
+lemma merge_transitions_7_5: "merge_transitions third_branch merge_7_5 6 5 5 5 5 (coin 50 100) 5 (coin 50 50) 4 (heuristics [third_trace, second_trace, first_trace]) = Some heuristics_7_5"
+  apply (rule merge_transitions_heuristic)
+  using coin_50_50_cant_directly_subsume_coin_50_100 apply blast
+  using coin_50_100_cant_directly_subsume_coin_50_50 apply blast
+  by eval
 
-lemma step_pta_select_coke: "step (tm pta) 0 Map.empty (STR ''select'') [(Str ''coke'')] = Some ((select coke), 1, [], <>)"
-  apply (rule one_possible_step)
-    apply (rule possible_steps_singleton)
-    apply (simp add: Abs_ffilter Set.filter_def pta_def tm_def)
-  using implode_coke implode_pepsi
-  by auto
+lemma no_choice: "\<forall> n m. \<not>choice (select_initialise coke n) (select_initialise pepsi m)"
+  by (simp add: choice_def)
 
-  lemma posterior_select_drink: "posterior \<lbrakk>\<rbrakk> (select d) = \<lbrakk>\<rbrakk>"
-    apply (rule posterior_consistent_medial)
-      apply (simp add: medial_def List.maps_def pairs2context_def)
-     apply (simp add: consistent_def)
-     apply (rule_tac x="<I 1 := Str d>" in exI)
-     defer
-     apply (rule ext)
-     apply (simp add: remove_obsolete_constraints_def)
-    apply safe
-      apply (simp add: cval_def)
-     apply (simp add: cval_true)
-    apply (case_tac r)
-       apply (simp add: cval_true)
-      apply (case_tac x2)
-    using cval_def
-    by auto
-
-lemma coin_100_100_not_directly_subsumes_coin_general: "\<not> directly_subsumes (tm pta) (tm merge_5_2) 8 (coin 100 100) coin_general \<and>
-                                                        \<not> directly_subsumes (tm pta) (tm merge_5_2) 1 coin_general (coin 100 100)"
+lemma nondeterministic_pairs_heuristics_7_5: "nondeterministic_pairs heuristics_7_5 = {||}"
 proof-
-  have select_pepsi: "step (tm merge_5_2) 0 Map.empty STR ''select'' [EFSM.Str pepsi] = Some (select pepsi, 7, [], <>)"
-    apply (rule one_possible_step)
-      defer
-      apply simp
-     apply simp
-    apply (simp add: possible_steps_alt Abs_ffilter tm_def merge_5_2_def Set.filter_def)
-    using implode_coke implode_pepsi
-    by auto
-  have step_merge_5_2_coin_7: "step (tm merge_5_2) 7 Map.empty STR ''coin'' [Num 50] = Some (coin_general, 1, [None], <>)"
-    apply (rule one_possible_step)
-      defer
-      apply simp
-     apply (rule ext)
-     apply simp
-    apply (simp add: possible_steps_alt Abs_ffilter Set.filter_def tm_def merge_5_2_def)
-    by auto
-  have posterior_coin_general: "posterior \<lbrakk>\<rbrakk> coin_general = \<lbrakk>\<rbrakk>"
-    apply (rule posterior_consistent_medial)
-      apply (simp add: medial_empty)
-     apply simp
-    apply (simp add: remove_obsolete_constraints_def)
-    apply (rule ext)
-    by (simp add: fprod_singletons)
-  have select_coke: "step (tm merge_5_2) 0 Map.empty STR ''select'' [EFSM.Str coke] = Some (select coke, 1, [], <>)"
-    apply (rule one_possible_step)
-      apply (simp add: possible_steps_alt Abs_ffilter Set.filter_def tm_def merge_5_2_def)
-    using implode_coke implode_pepsi
-    by auto
+  have union: "ffUnion ((\<lambda>s. state_nondeterminism s (outgoing_transitions s heuristics_7_5)) |`| Inference.S heuristics_7_5) = {|
+(5, (5, 8), (coin_general 2, 5), vend pepsi, 6), (5, (8, 5), (vend pepsi, 6), coin_general 2, 5), (1, (1, 4), (coin_general 1, 2), vend coke, 3),
+   (1, (4, 1), (vend coke, 3), coin_general 1, 2), (0, (1, 5), (select_initialise coke 1, 0), select_initialise pepsi 2, 1),
+   (0, (5, 1), (select_initialise pepsi 2, 1), select_initialise coke 1, 0)|}"
+    by eval
   show ?thesis
-    apply standard
-    apply (rule gets_us_to_and_not_subsumes)
-    apply (rule_tac x="[(STR ''select'', [Str pepsi]), (STR ''coin'', [Num 50])]" in exI)
-    apply standard
-     apply (simp add: accepts_trace_def)
-     apply (rule accepts.step)
-      apply (simp add: step_pta_select_pepsi)
-     apply (rule accepts.step)
-      apply (simp add: step_pta_coin50_7)
-     apply (simp add: accepts.base)
-    apply standard
-     apply (rule step_some)
-      apply (simp add: step_pta_select_pepsi)
-     apply (rule step_some)
-      apply (simp add: step_pta_coin50_7)
-     apply (simp add: gets_us_to.base)
-    apply (simp add: anterior_context_def)
-    apply (simp add: select_pepsi step_merge_5_2_coin_7)
-    apply (simp add: posterior_select_drink posterior_coin_general)
-    apply (simp add: subsumes_def)
-    using satisfies_context_empty apply fastforce
-    apply (rule gets_us_to_and_not_subsumes)
-    apply (rule_tac x="[(STR ''select'', [Str coke])]" in exI)
-    apply standard
-     apply (simp add: accepts_trace_def)
-     apply (rule accepts.step)
-      apply (simp add: step_pta_select_coke)
-     apply (simp add: accepts.base)
-    apply standard
-     apply (rule step_some)
-      apply (simp add: step_pta_select_coke)
-     apply (simp add: gets_us_to.base)
-    apply (simp add: anterior_context_def)
-    apply (simp add: select_coke posterior_select_drink)
-    apply (rule output_subsumption_violation)
-    apply simp
-    apply (rule_tac x="[Num 100]" in exI)
-    apply simp
-    apply (rule_tac x="<>" in exI)
-    by (simp add: satisfies_context_empty)
+    apply (rule nondeterministic_pairs)
+     apply (simp only: union)
+    apply (simp add: Abs_ffilter Set.filter_def)
+    apply clarify
+    apply (case_tac "ab = select_initialise coke 1")
+     apply (simp add: no_choice)
+    apply (case_tac "ab = select_initialise pepsi 2")
+     apply (simp add: no_choice choice_symmetry)
+    using choice_def by auto
 qed
 
-lemma pta_1_anterior_context: "accepts_trace (tm pta) p \<and> gets_us_to 1 (tm pta) 0 Map.empty p \<Longrightarrow> anterior_context (tm merge_5_2) p = \<lbrakk>\<rbrakk>"
-proof(induct p)
-  case Nil
-  then show ?case
-    by (simp add: anterior_context_def)
-next
-  have select_coke: "step (tm merge_5_2) 0 Map.empty STR ''select'' [EFSM.Str coke] = Some (select coke, 1, [], <>)"
-    apply (rule one_possible_step)
-      apply (simp add: possible_steps_alt Abs_ffilter Set.filter_def tm_def merge_5_2_def)
-    using implode_coke implode_pepsi
-    by auto
-  have posterior_coke: "posterior \<lbrakk>\<rbrakk> (select coke) = \<lbrakk>\<rbrakk>"
-    apply (rule posterior_consistent_medial)
-      apply (simp add: medial_def pairs2context_def List.maps_def)
-     apply (simp add: consistent_def)
-     apply (rule_tac x="<I 1 := Str coke>" in exI)
-     defer
-     apply simp
-    apply safe
-      apply (simp add: cval_def)
-     apply (simp add: cval_true)
-    apply (case_tac r)
-       apply (simp add: cval_def)
-      apply (case_tac x2)
-    using cval_def by auto
-  case (Cons a p)
-  then show ?case
-    apply (simp add: accepts_trace_def anterior_context_def)
-    apply (case_tac "a = (STR ''select'', [Str coke])")
-     apply (simp add: select_coke posterior_coke)
-    sorry
-qed
-
-lemma not_directly_subsumes_100_pta: "\<not> directly_subsumes (tm pta) (tm merge_5_2) 1 (coin 100 100) coin_general"
+lemma merge_third_branch: "merge third_branch 5 6 (heuristics [third_trace, second_trace, first_trace]) (satisfies {third_trace, second_trace, first_trace}) = Some heuristics_7_5"
 proof-
-  have select_coke: "step (tm merge_5_2) 0 Map.empty STR ''select'' [EFSM.Str coke] = Some (select coke, 1, [], <>)"
-    apply (rule one_possible_step)
-      apply (simp add: possible_steps_alt Abs_ffilter Set.filter_def tm_def merge_5_2_def)
-    using implode_coke implode_pepsi by auto
+  have arrives_5_merge_5_6: "arrives 5 merge_5_6 = 7"
+    by eval
+  have arrives_4_merge_5_6: "arrives 4 merge_5_6 = 5"
+    by eval
+  have leaves_5_third_branch: "leaves 5 third_branch = 6"
+    by eval
+  have leaves_4_third_branch: "leaves 4 third_branch = 5"
+    by eval
+  have leaves_5_merge_7_5: "leaves 5 merge_7_5 = 5"
+    by eval
+  have arrives_5_merge_7_5: "arrives 5 merge_7_5 = 5"
+    by eval
+  have arrives_4_merge_7_5: "arrives 4 merge_7_5 = 5"
+    by eval
+  have satisfies: "satisfies {third_trace, second_trace, first_trace} (tm heuristics_7_5)"
+    by eval
   show ?thesis
-    apply (rule gets_us_to_and_not_subsumes)
- apply (rule_tac x="[(STR ''select'', [Str coke])]" in exI)
-    apply standard
-     apply (simp add: accepts_trace_def)
-     apply (rule accepts.step)
-      apply (simp add: step_pta_select_coke)
-     apply (simp add: accepts.base)
-    apply standard
-     apply (rule step_some)
-      apply (simp add: step_pta_select_coke)
-     apply (simp add: gets_us_to.base)
-    apply (simp add: anterior_context_def)
-    apply (simp add: select_coke posterior_select_drink)
-    apply (rule output_subsumption_violation)
-    apply simp
-    apply (rule_tac x="[Num 100]" in exI)
-    apply simp
-    apply (rule_tac x="<>" in exI)
-    by (simp add: satisfies_context_empty)
+    apply (simp add: merge_def merge_5_6 nondeterministic_pairs_merge_5_6 sorted_list_of_fset_def)
+    apply (simp add: arrives_5_merge_5_6 arrives_4_merge_5_6 merge_7_5)
+    apply (simp add: leaves_5_third_branch leaves_4_third_branch leaves_5_merge_7_5 arrives_5_merge_7_5 arrives_4_merge_7_5)
+    apply (simp add: merge_transitions_7_5 nondeterministic_pairs_heuristics_7_5 deterministic_def)
+    by (simp add: satisfies)
 qed
 
-lemma minus: "{|(0::nat, (0::nat, 1::nat), select coke), (1, (0, 7), select pepsi), (2, (1, 2), coin_general), (3, (1, 5), coin 100 100),
-                   (4, (2, 3), coin50_initialise), (5, (3, 4), vend coke), (6, (5, 6), vend coke), (7, (7, 1), coin_general),
-                   (8, (1, 2), coin_general), (9, (2, 10), vend_initialise)|} |-|
-                 {|(2, (1, 2), coin_general)|} =
-{|(0, (0, 1), select coke),
-   (1, (0, 7), select pepsi),
-   (3, (1, 5), coin 100 100), (4, (2, 3), coin50_initialise),
-   (5, (3, 4), vend coke),
-   (6, (5, 6), vend coke),
-   (7, (7, 1), coin_general), (8, (1, 2), coin_general), (9, (2, 10), vend_initialise)|}"
-    apply (simp add: minus_fset_def fset_both_sides Abs_fset_inverse)
-    by auto
+lemma score_heuristics_7_5: "sorted_list_of_fset (score heuristics_7_5 naive_score) = [(2, 1, 5)]"
+  by eval
 
-lemma nondeterministic_pairs_heuristics_2_9_minus: "nondeterministic_pairs (heuristics_2_9 |-| {|(2, (1, 2), coin_general)|}) = {|
-(1, (2, 5), (coin_general, 8), coin 100 100, 3), (1, (5, 2), (coin 100 100, 3), coin_general, 8)
+lemma merge_1_5: "merge_states 1 5 heuristics_7_5 = merge_1_5"
+  by eval
+
+lemma nondeterministic_pairs_merge_1_5: "nondeterministic_pairs merge_1_5 = {|
+(1, (1, 1), (coin_general 1, 2), coin_general 2, 5),
+(1, (4, 8), (vend coke, 3), vend pepsi, 6),
+(1, (1, 1), (coin_general 2, 5), coin_general 1, 2),
+(1, (8, 4), (vend pepsi, 6), vend coke, 3)
 |}"
 proof-
-  have state_nondeterminism_1: "state_nondeterminism 1 {|(5, coin 100 100, 3), (2, coin_general, 8)|} = {|(1, (2, 5), (coin_general, 8), coin 100 100, 3), (1, (5, 2), (coin 100 100, 3), coin_general, 8)|}"
-    by eval
-  have state_nondeterminism_2: "state_nondeterminism 2 {|(3, coin50_initialise, 4), (10, vend_initialise, 9)|} = {|(2, (10, 3), (vend_initialise, 9), coin50_initialise, 4), (2, (3, 10), (coin50_initialise, 4), vend_initialise, 9)|}"
-    by eval
-  have state_nondeterminism_0:  "state_nondeterminism 0 {|(1, select coke, 0), (7, select pepsi, 1)|} = {|(0, (7, 1), (select pepsi, 1), select coke, 0), (0, (1, 7), (select coke, 0), select pepsi, 1)|}"
+  have union: "ffUnion ((\<lambda>s. state_nondeterminism s (outgoing_transitions s merge_1_5)) |`| Inference.S merge_1_5) = {|(1, (1, 4), (coin_general 1, 2), vend coke, 3), (1, (1, 1), (coin_general 1, 2), coin_general 2, 5), (1, (1, 8), (coin_general 1, 2), vend pepsi, 6),
+   (1, (4, 1), (vend coke, 3), coin_general 1, 2), (1, (4, 1), (vend coke, 3), coin_general 2, 5), (1, (4, 8), (vend coke, 3), vend pepsi, 6),
+   (1, (1, 1), (coin_general 2, 5), coin_general 1, 2), (1, (1, 4), (coin_general 2, 5), vend coke, 3), (1, (1, 8), (coin_general 2, 5), vend pepsi, 6),
+   (1, (8, 1), (vend pepsi, 6), coin_general 1, 2), (1, (8, 4), (vend pepsi, 6), vend coke, 3), (1, (8, 1), (vend pepsi, 6), coin_general 2, 5),
+   (0, (1, 1), (select_initialise coke 1, 0), select_initialise pepsi 2, 1), (0, (1, 1), (select_initialise pepsi 2, 1), select_initialise coke 1, 0)|}"
     by eval
   show ?thesis
-    apply (simp add: nondeterministic_pairs_def S_def heuristics_2_9_def)
-    apply (simp add: outgoing_transitions_def fimage_def minus Abs_fset_inverse)
-    apply (simp add: state_nondeterminism_0 state_nondeterminism_1 state_nondeterminism_2)
-    apply (simp add: ffUnion_def Abs_fset_inverse)
-    apply (simp add: Abs_ffilter Abs_fset_inverse Set.filter_def)
+    apply (rule nondeterministic_pairs)
+     apply (simp only: union)
+    apply (simp add: Abs_ffilter Set.filter_def)
     apply standard
      apply clarify
      apply simp
-     apply (case_tac "ab = coin_general")
-      apply simp
-     apply (case_tac "ab = vend_initialise")
-      apply (simp add: choice_def)
-    apply (case_tac "ab = coin50_initialise")
-      apply (simp add: choice_def)
+     apply (case_tac "ab = select_initialise coke 1")
+     apply (simp add: no_choice)
+    apply (case_tac "ab = select_initialise pepsi 2")
+     apply (simp add: no_choice choice_symmetry)
      apply simp
-     apply (meson choice_symmetry no_choice_select_coke_select_pepsi)
-    apply clarify
-    apply simp
-    using choice_coin_specific_coin_general choice_symmetry by blast
+     apply (case_tac "ab = vend coke")
+      apply (case_tac "ac = vend pepsi")
+       apply simp
+    using choice_def apply auto[1]
+     apply simp
+     apply (case_tac "ab = vend pepsi")
+     apply (case_tac "ac = vend coke")
+       apply simp
+    using choice_def apply auto[1]
+     apply simp
+     apply (case_tac "ac = vend coke")
+      apply (case_tac "ab = vend pepsi")
+       apply simp
+    using choice_def apply auto[1]
+
+     apply (case_tac "ac = vend pepsi")
+      apply (case_tac "ab = vend coke")
+       apply simp
+    using choice_def apply auto[1]
+     apply auto[1]
+    apply (simp add: choice_def)
+    by auto
 qed
 
-definition "merge_states_5_2_a = 
-{|(0, (0, 1), select coke),
-   (1, (0, 7), select pepsi),
-   (3, (1, 2), coin 100 100), (4, (2, 3), coin50_initialise),
-   (5, (3, 4), vend coke),
-   (6, (2, 6), vend coke),
-   (7, (7, 1), coin_general), (8, (1, 2), coin_general), (9, (2, 10), vend_initialise)|}"
-
-lemma merge_states_5_2_a: "merge_states 5 2 (heuristics_2_9 |-| {|(2, (1, 2), coin_general)|}) = merge_states_5_2_a"
+lemma merge_ar6_ar3: "merge_states (arrives 6 merge_1_5) (arrives 3 merge_1_5) merge_1_5 = merge_ar6_ar3"
   by eval
 
-lemma "merge_transitions pta merge_states_5_2_a 1 8 1 2 2 (coin 100 100) 3 coin_general 8 heuristics = None"
-  apply (simp add: merge_transitions_def)
-  oops
+lemma merge_transitions_heuristics_7_5: "merge_transitions heuristics_7_5 merge_ar6_ar3 5 1 1 4 4 (vend pepsi) 6 (vend coke) 3 (heuristics [third_trace, second_trace, first_trace]) = Some heuristics_1_0"
+  apply (rule merge_transitions_heuristic)
+    apply (simp add: cant_directly_subsume no_subsumption_vend_coke_vend_pepsi)
+   apply (simp add: cant_directly_subsume vend_pepsi_not_subsumes_vend_coke)
+  by eval
 
-lemma "merge pta 1 8 heuristics (satisfies (set traces)) = None"
+lemma nondeterministic_pairs_heuristics_1_0: "nondeterministic_pairs heuristics_1_0 = {|
+(0, (1, 5), (select_general_1, 0), select_initialise pepsi 2, 1),
+(0, (5, 1), (select_initialise pepsi 2, 1), select_general_1, 0)
+|}"
 proof-
-  have arrives_8_merged_1_8:  "arrives 8 merged_1_8 = 9"
+  have union: "ffUnion ((\<lambda>s. state_nondeterminism s (outgoing_transitions s heuristics_1_0)) |`| Inference.S heuristics_1_0) = {|
+(5, (5, 8), (coin_general 2, 4), vend pepsi, 5), (5, (8, 5), (vend pepsi, 5), coin_general 2, 4), (1, (1, 4), (coin_general 1, 2), vend_general_1, 3),
+   (1, (4, 1), (vend_general_1, 3), coin_general 1, 2), (0, (1, 5), (select_general_1, 0), select_initialise pepsi 2, 1),
+   (0, (5, 1), (select_initialise pepsi 2, 1), select_general_1, 0)|}"
     by eval
-  have arrives_2_merged_1_8: "(arrives 2 merged_1_8) = 2"
-    by eval
-  have leaves_8_merged_2_9:  "leaves 8 merged_2_9 = 1"
-    by eval
-  have heuristics_merged_2_9: "heuristics 8 2 1 merged_2_9 pta = Some heuristics_2_9"
-    by eval
-  have arrives_3_heuristics_2_9: "arrives 3 heuristics_2_9 = 5"
-    by eval
-  have arrives_8_heuristics_2_9: "arrives 8 heuristics_2_9 = 2"
-    by eval
-  have leaves_3_pta: "leaves 3 pta = 1"
-    by eval
-  have leaves_8_pta: "leaves 8 pta = 8"
-    by eval
-  have leaves_3_merge_5_2: "leaves 3 merge_5_2 = 1"
-    by eval
-  have arrives_3_merge_5_2: "arrives 3 merge_5_2 = 2"
-    by eval
-  have arrives_8_merge_5_2: "arrives 8 merge_5_2 = 2"
-    by eval
-  have merge_transitions_coin_100_100_general_none: "merge_transitions pta merge_5_2 1 8 1 2 2 (coin 100 100) 3 coin_general 8 heuristics = None"
-    proof-
-      show ?thesis
-        apply (simp add: merge_transitions_def coin_100_100_not_directly_subsumes_coin_general)
-        by eval
-    qed
-    have arrives_2_heuristics_2_9: "arrives 2 heuristics_2_9 = 2"
-      by eval
-    have leaves_2_pta: "leaves 2 pta = 1"
-      by eval
-    have arrives_2_merge_5_2: "arrives 2 merge_5_2 = 2"
-      by eval
-    have merge_transitions_2: "merge_transitions pta merge_5_2 1 1 1 2 2 (coin 100 100) 3 coin_general 2 heuristics = None"
-      apply (simp add: merge_transitions_def)
-      apply (simp add: coin_100_100_not_directly_subsumes_coin_general not_directly_subsumes_100_pta)
-      by eval
-    have leaves_8_merge_5_2: "leaves 8 merge_5_2 = 1"
-      by eval
-    have merge_transitions_3: "merge_transitions pta merge_5_2 8 1 1 2 2 coin_general 8 (coin 100 100) 3 heuristics = None"
-      apply (simp add: merge_transitions_def)
-      apply (simp add: coin_100_100_not_directly_subsumes_coin_general not_directly_subsumes_100_pta)
-      by eval
-    have leaves_2_merge_5_2: "leaves 2 merge_5_2 = 1"
-      by eval
-    have merge_transitions_4: "merge_transitions pta merge_5_2 1 1 1 2 2 coin_general 2 (coin 100 100) 3 heuristics = None"
-      apply (simp add: merge_transitions_def)
-      apply (simp add: coin_100_100_not_directly_subsumes_coin_general not_directly_subsumes_100_pta)
-      by eval
-    have leaves_8_heuristics_2_9: "leaves 8 heuristics_2_9 = 1"
-      by eval
-    have arrives_8_heuristics_2_9: "arrives 8 heuristics_2_9 = 2"
-      by eval
-    have arrives_2_heuristics_2_9: "arrives 2 heuristics_2_9 = 2"
-      by eval
-    have merge_transitions_general_general: "merge_transitions pta heuristics_2_9 8 1 1 2 2 coin_general 8 coin_general 2 heuristics = Some (heuristics_2_9 |-| {|(2, (1, 2), coin_general)|})"
-      apply (simp add: merge_transitions_def)
-      apply (simp add: directly_subsumes_def transition_subsumes_self)
-      apply (simp add: replace_transition_def heuristics_2_9_def)
-      by eval
-    have arrives_3_minus:  "arrives 3 (heuristics_2_9 |-| {|(2, (1, 2), coin_general)|}) = 5"
-      by eval
-    have arrives_8_minus: "(arrives 8 (heuristics_2_9 |-| {|(2, (1, 2), coin_general)|})) = 2"
-      by eval
-    have leaves_3_merge_states_5_2_a: "leaves 3 merge_states_5_2_a = 1"
-      by eval
-    have arrives_3_merge_states_5_2_a: "arrives 3 merge_states_5_2_a = 2"
-      by eval
-    have arrives_8_merge_states_5_2_a: "arrives 8 merge_states_5_2_a = 2"
-      by eval
   show ?thesis
-    apply (simp add: merge_def merge_states_1_8 nondeterministic_pairs_merged_1_8 sorted_list_of_fset_def)
-    apply (simp add: arrives_8_merged_1_8 arrives_2_merged_1_8 merge_states_2_9)
-    apply (simp add: merge_transitions_def coin_50_100_cant_directly_subsume_coin_50_50 coin_50_50_cant_directly_subsume_coin_50_100)
-    apply (simp add: leaves_8_merged_2_9 heuristics_merged_2_9)
-    apply (simp add: nondeterministic_pairs_heuristics_2_9 sorted_list_of_fset_def)
+    apply (rule nondeterministic_pairs)
+     apply (simp only: union)
+    apply (simp add: Abs_ffilter Set.filter_def)
+    apply standard
+     apply clarify
+     apply simp
+     apply (case_tac "ab = select_general_1")
+      apply simp
+     apply (case_tac "ab = select_initialise pepsi 2")
+      apply simp
+    using choice_def by auto
+qed
 
-    apply (simp add: arrives_3_heuristics_2_9 arrives_8_heuristics_2_9)
-    apply (simp add: merge_5_2)
-    apply (simp add: leaves_3_pta leaves_8_pta leaves_3_merge_5_2 arrives_3_merge_5_2 arrives_8_merge_5_2)
-    apply (simp add: merge_transitions_coin_100_100_general_none)
+lemma merge_a1_a0: "merge_states (arrives 1 heuristics_1_0) (arrives 0 heuristics_1_0) heuristics_1_0 = merge_a1_a0"
+  by eval
 
-    apply (simp add: arrives_3_heuristics_2_9 arrives_2_heuristics_2_9)
-    apply (simp add: merge_5_2)
-    apply (simp add: leaves_3_pta leaves_2_pta leaves_3_merge_5_2 arrives_3_merge_5_2 arrives_2_merge_5_2)
-    apply (simp add: merge_transitions_2)
+lemma no_direct_subsumption_pepsi_general: "\<not> directly_subsumes (tm heuristics_7_5) (tm merge_a1_a0) 0 (select_initialise pepsi 2) select_general_1"
+  apply (rule gets_us_to_and_not_subsumes)
+  apply (rule_tac x="[]" in exI)
+  apply standard
+   apply (simp add: accepts_trace_def accepts.base)
+  apply standard
+   apply (simp add: gets_us_to.base)
+  apply (simp add: anterior_context_def)
+  apply (rule medial_subsumption_violation)
+  apply simp
+  apply (rule_tac x="V (I 1)" in exI)
+  apply (rule_tac x="<>" in exI)
+  apply (simp add: medial_empty cval_true)
+  apply (simp add: medial_def cval_true)
+  by (simp add: pairs2context_def List.maps_def cval_def)
 
-    apply (simp add: arrives_3_heuristics_2_9 arrives_8_heuristics_2_9)
-    apply (simp add: merge_5_2)
-    apply (simp add: leaves_3_pta leaves_8_pta leaves_8_merge_5_2 arrives_3_merge_5_2 arrives_8_merge_5_2)
-    apply (simp add: merge_transitions_3)
+lemma not_directly_subsumes_general_pepsi: "\<not>directly_subsumes (tm heuristics_7_5) (tm merge_a1_a0) 0 select_general_1 (select_initialise pepsi 2)"
+proof-
+  have posterior_select_pepsi: "(posterior \<lbrakk>\<rbrakk> (select_initialise pepsi 2)) = \<lbrakk>V (R 2) \<mapsto> {|Eq (Num 0)|}\<rbrakk>"
+    apply (rule posterior_consistent_medial)
+      apply (simp add: medial_def List.maps_def pairs2context_def)
+     apply (simp add: consistent_def)
+     apply (rule_tac x="<I 1 := Str ''pepsi''>" in exI)
+     apply clarify
+     apply standard+
+    apply clarify
+       apply (simp add: cval_def implode_pepsi)
+      apply clarify
+      apply (simp add: cval_def)
+     apply (case_tac r)
+        apply (simp add: cval_true)
+       apply (case_tac x2)
+        apply (simp add: cval_def)+
+    apply (rule ext)
+    by (simp add: remove_obsolete_constraints_def)
+  have consistent_post_select_p: " consistent (posterior \<lbrakk>\<rbrakk> (select_initialise pepsi 2))"
+    apply (simp add: posterior_select_pepsi consistent_def)
+    apply (rule_tac x="<R 2 := Num 0>" in exI)
+    apply (simp add: cval_def)
+    apply clarify
+    apply (case_tac r)
+       apply (simp add: cval_true)
+      apply (case_tac x2)
+    using cval_def by auto
+  have posterior_select_general: "posterior \<lbrakk>\<rbrakk> select_general_1 = \<lbrakk>V (R 3) \<mapsto> {|Bc True|}, V (R 1) \<mapsto> {|Eq (Num 0)|}\<rbrakk>"
+    apply (rule posterior_consistent_medial)
+      apply (simp add: medial_def List.maps_def pairs2context_def)
+     apply (simp add: consistent_def)
+     apply (rule_tac x="<I 1 := Str ''pepsi''>" in exI)
+     apply clarify
+     apply (case_tac r)
+        apply (simp add: cval_true)
+       apply (case_tac x2)
+        apply (simp add: cval_def)+
+    apply (rule ext)
+    by (simp add: remove_obsolete_constraints_def)
+  have consistent_posterior_select_g: "consistent (posterior \<lbrakk>\<rbrakk> select_general_1)"
+    apply (simp add: posterior_select_general consistent_def)
+    apply (rule_tac x="<R 1 := Num 0>" in exI)
+    apply (simp add: cval_true)
+    apply clarify
+     apply (case_tac r)
+        apply (simp add: cval_true)
+       apply (case_tac x2)
+    by (simp add: cval_def)+
+  have not_medial: "\<not>(\<exists>r i. fBall (medial \<lbrakk>\<rbrakk> [gexp.Eq (V (I 1)) (L (value.Str pepsi))] r) (\<lambda>c. cval c r i = true) \<and> fBex (\<lbrakk>\<rbrakk> r) (\<lambda>x. cval x r i \<noteq> true))"
+    apply (simp add: medial_def pairs2context_def List.maps_def)
+    by auto
+  have consistent_medial: "consistent (medial \<lbrakk>\<rbrakk> [gexp.Eq (V (I 1)) (L (value.Str pepsi))])"
+    apply (simp add: medial_def List.maps_def pairs2context_def consistent_def)
+    apply (rule_tac x="<I 1 := Str ''pepsi''>" in exI)
+    apply safe
+      apply (simp add: cval_def implode_pepsi)
+     apply (simp add: cval_true)
+    apply (case_tac r)
+     apply (simp add: cval_true)
+       apply (case_tac x2)
+    by (simp add: cval_def)+
+  have posterior_separate: "posterior_separate \<lbrakk>\<rbrakk> [gexp.Eq (V (I 1)) (L (value.Str pepsi))] [(R 3, V (I 1)), (R 1, L (Num 0))] = \<lbrakk>V (R 3) \<mapsto> {|Eq (Str ''pepsi''), Bc True|}, V (R 1) \<mapsto> {|Eq (Num 0)|}\<rbrakk>"
+    apply (simp add: posterior_separate_def Let_def)
+    apply standard
+     apply clarify
+     apply (rule ext)
+     apply (simp add: remove_obsolete_constraints_def)
+     apply (simp add: medial_def List.maps_def pairs2context_def)
+     apply standard
+      apply auto[1]
+     apply (simp add: implode_pepsi)
+    by (simp add: consistent_medial)
+  show ?thesis
+  apply (rule gets_us_to_and_not_subsumes)
+  apply (rule_tac x="[]" in exI)
+ apply standard
+   apply (simp add: accepts_trace_def accepts.base)
+  apply standard
+   apply (simp add: gets_us_to.base)
+  apply (simp add: anterior_context_def)
+    apply (simp add: subsumes_def medial_empty consistent_post_select_p consistent_posterior_select_g)
+    apply (simp add: not_medial)
+    apply (simp add: posterior_select_pepsi posterior_separate)
+    apply (rule_tac x="V (R 2)" in exI)
+    apply simp
+    apply (rule_tac x="<>" in exI)
+    by (simp add: cval_def)
+qed
 
-    apply (simp add: arrives_3_heuristics_2_9 arrives_2_heuristics_2_9)
-    apply (simp add: merge_5_2)
-    apply (simp add: leaves_3_pta leaves_2_pta arrives_3_merge_5_2 arrives_2_merge_5_2 leaves_2_merge_5_2)
-    apply (simp add: merge_transitions_4)
+lemma increment_none: "insert_increment 1 0 0 merge_a1_a0 heuristics_7_5 = None"
+  by eval
 
-    apply (simp add: arrives_2_heuristics_2_9 arrives_8_heuristics_2_9)
-    apply (simp add: merge_states_reflexive)
-    apply (simp add: leaves_8_pta leaves_2_pta leaves_8_heuristics_2_9 arrives_8_heuristics_2_9 arrives_2_heuristics_2_9)
-    apply (simp add:merge_transitions_general_general)
+lemma "heuristics [third_trace, second_trace, first_trace] 1 0 0 merge_a1_a0 heuristics_7_5 = Some heuristics_1_0"
+  apply (simp add: heuristics_def increment_none del: insert_increment.simps)
 
-    apply (simp add: nondeterministic_pairs_heuristics_2_9_minus sorted_list_of_fset_def)
-    apply (simp add: arrives_3_minus arrives_8_minus merge_states_5_2_a)
-    apply (simp add: leaves_3_pta leaves_8_pta leaves_3_merge_states_5_2_a arrives_3_merge_states_5_2_a
-                     arrives_8_merge_states_5_2_a)
+lemma merge_transitions_a1_a0: "merge_transitions heuristics_7_5 merge_a1_a0 0 0 0 1 1 (select_initialise pepsi 2) 1 select_general_1 0
+                (heuristics [third_trace, second_trace, first_trace]) = Some heuristics_1_0"
+  apply (simp add: merge_transitions_def no_direct_subsumption_pepsi_general not_directly_subsumes_general_pepsi)
+  by eval
+
+lemma not_directly_subsumes_general_pepsi_2: "\<not> directly_subsumes (tm heuristics_7_5) (tm merge_a1_a0) (leaves 1 heuristics_7_5) select_general_1 (select_initialise pepsi 2)"
+proof-
+  have leaves_1_heuristics_7_5: "leaves 1 heuristics_7_5 = 0"
+    by eval
+  have medial: "medial \<lbrakk>\<rbrakk> [gexp.Eq (V (I 1)) (L (value.Str pepsi))] = \<lbrakk>V (I 1) \<mapsto> {|Eq (Str ''pepsi''), Bc True|}\<rbrakk>"
+    apply (rule ext)
+    by (simp add: medial_def List.maps_def pairs2context_def implode_pepsi)
+  have consistent_medial: "consistent \<lbrakk>V (I 1) \<mapsto> {|cexp.Eq (EFSM.Str ''pepsi''), cexp.Bc True|}\<rbrakk>"
+    apply (simp add: consistent_def)
+    apply (rule_tac x="<I 1 \<mapsto> Str ''pepsi''>" in exI)
+    apply clarify
+    apply (simp add: cval_def)
+    apply (case_tac r)
+       apply (simp add: cval_true)
+      apply (case_tac x2)
+    using cval_def by auto
+  have violation: "(\<exists>r i. fBall (posterior_separate \<lbrakk>\<rbrakk> [gexp.Eq (V (I 1)) (L (value.Str pepsi))] [(R 3, V (I 1)), (R 1, L (Num 0))] r) (\<lambda>c. cval c r i = true) \<and>
+           fBex (posterior \<lbrakk>\<rbrakk> (select_initialise pepsi 2) r) (\<lambda>x. cval x r i \<noteq> true) \<and> posterior \<lbrakk>\<rbrakk> (select_initialise pepsi 2) r \<noteq> {|Undef|})"
+    apply (simp add: posterior_def posterior_separate_def Let_def medial consistent_medial)
+    apply (simp add: remove_obsolete_constraints_def)
+    apply (rule_tac x="V (R 2)" in exI)
+    apply simp
+    apply (rule_tac x="<>" in exI)
+    by (simp add: cval_def)
+  show ?thesis
+  apply (rule gets_us_to_and_not_subsumes)
+  apply (rule_tac x="[]" in exI)
+     apply (simp add: accepts_trace_def accepts.base)
+     apply (simp add: leaves_1_heuristics_7_5 gets_us_to.base)
+    apply (simp add: anterior_context_def)
+    by (simp add: subsumes_def violation)
+qed
+
+lemma not_directly_subsumes_initialise_general: "\<not> directly_subsumes (tm heuristics_7_5) (tm merge_a1_a0) (leaves 0 heuristics_7_5) (select_initialise pepsi 2) select_general_1"
+proof-
+  have leaves_0_heuristics_7_5: "leaves 0 heuristics_7_5 = 0"
+    by eval
+ have medial: "medial \<lbrakk>\<rbrakk> [gexp.Eq (V (I 1)) (L (value.Str pepsi))] = \<lbrakk>V (I 1) \<mapsto> {|Eq (Str ''pepsi''), Bc True|}\<rbrakk>"
+    apply (rule ext)
+    by (simp add: medial_def List.maps_def pairs2context_def implode_pepsi)
+  have consistent_medial: "consistent \<lbrakk>V (I 1) \<mapsto> {|cexp.Eq (EFSM.Str ''pepsi''), cexp.Bc True|}\<rbrakk>"
+    apply (simp add: consistent_def)
+    apply (rule_tac x="<I 1 \<mapsto> Str ''pepsi''>" in exI)
+    apply clarify
+    apply (simp add: cval_def)
+    apply (case_tac r)
+       apply (simp add: cval_true)
+      apply (case_tac x2)
+    using cval_def by auto
+  have violation: "(\<exists>r i. fBall (posterior_separate \<lbrakk>\<rbrakk> [gexp.Eq (V (I 1)) (L (value.Str pepsi))] [(R 2, L (Num 0))] r) (\<lambda>c. cval c r i = true) \<and>
+           fBex (posterior \<lbrakk>\<rbrakk> select_general_1 r) (\<lambda>x. cval x r i \<noteq> true) \<and> posterior \<lbrakk>\<rbrakk> select_general_1 r \<noteq> {|Undef|})"
+    apply (simp add: posterior_def posterior_separate_def Let_def medial consistent_medial medial_empty)
+    apply (simp add: remove_obsolete_constraints_def)
+    apply (rule_tac x="V (R 1)" in exI)
+    apply simp
+    apply (rule_tac x="<>" in exI)
+    by (simp add: cval_def)
+  show ?thesis
+  apply (rule gets_us_to_and_not_subsumes)
+  apply (rule_tac x="[]" in exI)
+    apply (simp add: accepts_trace_def accepts.base leaves_0_heuristics_7_5 gets_us_to.base)
+    by (simp add: subsumes_def anterior_context_def violation)
+qed
+
+lemma insert_increment_none: "insert_increment 1 0 (leaves 1 merge_a1_a0) merge_a1_a0 heuristics_7_5 = None"
+  by eval
+
+lemma "merge heuristics_7_5 1 5 (heuristics [third_trace, second_trace, first_trace]) (satisfies {third_trace, second_trace, first_trace}) = Some e"
+proof-
+  have sorted_list_of_fset:  "sorted_list_of_fset (nondeterministic_pairs merge_1_5) =
+[(1, (1, 1), (coin_general 1, 2), coin_general 2, 5), (1, (1, 1), (coin_general 2, 5), coin_general 1, 2), (1, (4, 8), (vend coke, 3), vend pepsi, 6),
+  (1, (8, 4), (vend pepsi, 6), vend coke, 3)]"
+  apply (simp add: nondeterministic_pairs_merge_1_5)
+    by eval
+  have leaves_6_heuristics_7_5: "leaves 6 heuristics_7_5 = 5"
+    by eval
+  have leaves_3_heuristics_7_5: "leaves 3 heuristics_7_5 = 1"
+    by eval
+  have leaves_6_merge_ar6_ar3: "leaves 6 merge_ar6_ar3 = 1"
+    by eval
+  have arrives_6_merge_ar6_ar3: "arrives 6 merge_ar6_ar3 = 4"
+    by eval
+  have arrives_3_merge_ar6_ar3: "arrives 3 merge_ar6_ar3 = 4"
+    by eval
+  have leaves_1_heuristics_7_5: "leaves 1 heuristics_7_5 = 0"
+    by eval
+  have leaves_0_heuristics_7_5: "leaves 0 heuristics_7_5 = 0"
+    by eval
+  have leaves_1_merge_a1_a0: "leaves 1 merge_a1_a0 = 0"
+    by eval
+  have arrives_1_merge_a1_a0: "arrives 1 merge_a1_a0 = 1"
+    by eval
+  have arrives_0_merge_a1_a0: "arrives 0 merge_a1_a0 = 1"
+    by eval
+  show ?thesis
+    apply (simp add: merge_def merge_1_5 sorted_list_of_fset merge_ar6_ar3)
+    apply (simp add: leaves_6_heuristics_7_5 leaves_3_heuristics_7_5 leaves_6_merge_ar6_ar3 arrives_6_merge_ar6_ar3 arrives_3_merge_ar6_ar3)
+    apply (simp add: merge_transitions_heuristics_7_5)
+
+    apply (simp add: nondeterministic_pairs_heuristics_1_0 sorted_list_of_fset_def merge_a1_a0)
+    apply (simp add: leaves_1_heuristics_7_5 leaves_0_heuristics_7_5  arrives_1_merge_a1_a0 leaves_1_merge_a1_a0 arrives_0_merge_a1_a0)
+    apply (simp add: merge_transitions_a1_a0)
+
+    apply (simp add: nondeterministic_pairs_heuristics_1_0 sorted_list_of_fset_def merge_a1_a0)
+    apply (simp add: leaves_1_heuristics_7_5 leaves_0_heuristics_7_5  arrives_1_merge_a1_a0 leaves_1_merge_a1_a0 arrives_0_merge_a1_a0)
+    apply (simp add: merge_transitions_a1_a0)
+
+lemma "iterative_learn traces naive_score heuristics = (tm final)"
+  apply (simp add: iterative_learn_def)
+  apply (rule tm_same)
+  apply (simp add: traces_alt first_branch score_first_branch)
+  apply (simp add: merge_first_branch_1_2 score_first_branch_initialise)
+  apply (simp add: second_branch score_second_branch)
+  apply (simp add: merge_first_branch_1_2 score_first_branch_initialise)
+  apply (simp add: second_branch third_branch)
+  apply (simp add: score_third_branch merge_third_branch)
+  apply (simp add: score_heuristics_7_5)
 
 
-lemma "learn traces naive_score heuristics = (tm final)"
-  apply (simp add: learn_def build_pta scoring_1)
 
 
 end
