formal/inference/InferenceTestEFSMs.thy
@@ -1,0 +1,36 @@
+theory InferenceTestEFSMs
+imports Learn_EFSM
+begin
+
+abbreviation "coin_general r \<equiv> \<lparr>Label = STR ''coin'', Arity = 1, Guard = [], Outputs = [Plus (V (R r)) (V (I 1))], Updates = [(R r, Plus (V (R r)) (V (I 1)))]\<rparr>"
+abbreviation "vend_initialise \<equiv> \<lparr>Label = STR ''vend'', Arity = 0, Guard = [], Outputs = [L (value.Str STR ''pepsi'')], Updates = [(R 1, L (Num 0))]\<rparr>"
+abbreviation "coin50_initialise \<equiv> \<lparr>Label = STR ''coin'', Arity = 1, Guard = [gexp.Eq (V (I 1)) (L (Num 50))], Outputs = [L (Num 100)], Updates = [(R 1, L (Num 0))]\<rparr>"
+abbreviation "select_initialise d r  \<equiv> \<lparr>Label = STR ''select'', Arity = 1, Guard = [gexp.Eq (V (I 1)) (L (value.Str d))], Outputs = [], Updates = [(R r, L (Num 0))]\<rparr>"
+
+definition "first_branch = {|(0, (0, 1), select coke), (1, (1, 2), coin 50 50), (2, (2, 3), coin 50 100), (3, (3, 4), vend coke)|}"
+definition "merge_1_2 =    {|(0, (0, 1), select coke), (1, (1, 1), coin 50 50), (2, (1, 3), coin 50 100), (3, (3, 4), vend coke)|}"
+definition "merge_3_1 =    {|(0, (0, 1), select coke), (1, (1, 1), coin 50 50), (2, (1, 1), coin 50 100), (3, (1, 4), vend coke)|}"
+definition "first_branch_initialise = {|(0, (0, 1), select_initialise coke 1), (2, (1, 1), coin_general 1), (3, (1, 4), vend coke)|}"
+abbreviation "select_general_1 \<equiv> \<lparr>Label = STR ''select'', Arity = 1, Guard = [], Outputs = [], Updates = [(R 3, V (I 1)), (R 1, L (Num 0))]\<rparr>"
+abbreviation "vend_general_1 \<equiv> \<lparr>Label = STR ''vend'', Arity = 0, Guard = [], Outputs = [V (R 3)], Updates = []\<rparr>"
+
+definition "second_branch = {|(0, (0, 1), select_initialise coke 1), (1, (1, 1), coin_general 1), (2, (1, 4), vend coke)|}"
+
+definition "third_branch =              {|(0, (0, 1), select_initialise coke 1), (2, (1, 1), coin_general 1), (3, (1, 4), vend coke),
+                                           (1, (0, 5), select pepsi), (4, (5, 6), coin 50 50), (5, (6, 7), coin 50 100), (6, (7, 8), vend pepsi)|}"
+definition "merge_5_6 =                 {|(0, (0, 1), select_initialise coke 1), (2, (1, 1), coin_general 1), (3, (1, 4), vend coke),
+                                           (1, (0, 5), select pepsi), (4, (5, 5), coin 50 50), (5, (5, 7), coin 50 100), (6, (7, 8), vend pepsi)|}"
+definition "merge_7_5 =                 {|(0, (0, 1), select_initialise coke 1), (2, (1, 1), coin_general 1), (3, (1, 4), vend coke),
+                                           (1, (0, 5), select pepsi), (4, (5, 5), coin 50 50), (5, (5, 5), coin 50 100), (6, (5, 8), vend pepsi)|}"
+definition "heuristics_7_5 =            {|(0, (0, 1), select_initialise coke 1), (2, (1, 1), coin_general 1), (3, (1, 4), vend coke),
+                                           (1, (0, 5), select_initialise pepsi 2), (5, (5, 5), coin_general 2), (6, (5, 8), vend pepsi)|}"
+definition "merge_1_5 =                 {|(0, (0, 1), select_initialise coke 1), (2, (1, 1), coin_general 1), (3, (1, 4), vend coke),
+                                           (1, (0, 1), select_initialise pepsi 2), (5, (1, 1), coin_general 2), (6, (1, 8), vend pepsi)|}"
+definition "merge_ar6_ar3 =            {|(0, (0, 1), select_initialise coke 1), (2, (1, 1), coin_general 1), (3, (1, 4), vend coke),
+                                          (1, (0, 1), select_initialise pepsi 2), (5, (1, 1), coin_general 2), (6, (1, 4), vend pepsi)|}"
+definition "heuristics_1_0 =           {|(0, (0, 1), select_general_1), (2, (1, 1), coin_general 1), (3, (1, 4), vend_general_1),
+                                          (1, (0, 5), select_initialise pepsi 2), (4, (5, 5), coin_general 2), (5, (5, 8), vend pepsi)|}"
+definition "merge_a1_a0 =              {|(0, (0, 1), select_general_1), (2, (1, 1), coin_general 1), (3, (1, 4), vend_general_1),
+                                          (1, (0, 1), select_initialise pepsi 2), (4, (1, 1), coin_general 2), (5, (1, 8), vend pepsi)|}"
+
+end
